rework judgment

Fomega/Basic/Weaken.lean
@@ -14,87 +14,99 @@ namespace Fomega.Proof
   cases x <;> simp at *
   case _ x => rw [<-h x]; simp
 
-  theorem rename (r : Ren) : Γ ⊢ t : A ->
+  -- theorem rename (r : Ren) : Γ ⊢ t : A ->
+  --   (∀ x, [r#r](Γ d@ x) = Δ d@ (r x)) ->
+  --   Δ ⊢ ([r#r]t) : ([r#r]A)
+
+  @[simp]
+  abbrev idx_ren (r : Ren) : JudgmentIndex v -> JudgmentIndex v :=
+    match v with
+    | .prf => λ (t, A) => ([r#r]t, [r#r]A)
+    | .wf => λ () => ()
+
+  theorem rename (r : Ren) :
+    Judgment v Γ idx ->
+    ⊢ Δ ->
     (∀ x, [r#r](Γ d@ x) = Δ d@ (r x)) ->
-    Δ ⊢ ([r#r]t) : ([r#r]A)
+    Judgment v Δ (idx_ren r idx)
   := by
-  intro j h
+  intro j h1 h2
   induction j generalizing Δ r
+  case nil => simp; apply h1
+  case cons => simp; apply h1
   case ax ih =>
-    replace ih := ih 0 r h
-    rw [h 0] at ih; simp at ih
-    have lem := ctx_wf ih
-    cases lem
-    case _ f lem =>
-      constructor; apply lem
-  case var x _ _ ih =>
-    simp at *; rw [h x]; constructor
-    rw [<-(h x)]; apply ih r h
+    replace ih := ih r h1 h2
+    simp at *; constructor; apply ih
+  case var x K T j1 j2 ih =>
+    simp at *; rw [j2, h2 x]; constructor
+    rw [<-(h2 x)]; apply ih r h1 h2; rfl
   case pi Γ' A' K B _j1 _j2 ih1 ih2 =>
     simp; constructor
-    case _ => apply ih1 r h
+    case _ => apply ih1 r h1 h2
     case _ =>
-      replace ih2 := @ih2 ([r#r]A' :: Δ) (Term.Ren.lift r) (rename_lift r A' h)
+      have lem : ⊢ ([r#r]A' :: Δ) := by constructor; apply h1; apply ih1 r h1 h2
+      replace ih2 := @ih2 ([r#r]A' :: Δ) (Term.Ren.lift r) lem (rename_lift r A' h2)
       simp at ih2; exact ih2
   case tpi Γ' A' B _j1 _j2 ih1 ih2 =>
     simp; constructor
-    case _ => apply ih1 r h
+    case _ => apply ih1 r h1 h2
     case _ =>
-      replace ih2 := @ih2 ([r#r]A' :: Δ) (Term.Ren.lift r) (rename_lift r A' h)
+      have lem : ⊢ ([r#r]A' :: Δ) := by constructor; apply h1; apply ih1 r h1 h2
+      replace ih2 := @ih2 ([r#r]A' :: Δ) (Term.Ren.lift r) lem (rename_lift r A' h2)
       simp at ih2; exact ih2
-  case lam Γ' A' B K t _j1 _j2 ih1 ih2 =>
+  case lam Γ A B K t j1 j2 ih1 ih2  =>
     simp; constructor
-    case _ => simp at ih1; apply ih1 r h
     case _ =>
-      replace ih2 := @ih2 ([r#r]A' :: Δ) (Term.Ren.lift r) (rename_lift r A' h)
+      have lem : ⊢ ([r#r]A :: Δ) := by
+        constructor; apply h1; replace ih1 := ih1 r h1 h2; simp at ih1
+      replace ih1 := @ih1 ([r#r]A :: Δ) (Term.Ren.lift r) lem (rename_lift r A h2)
+      simp at ih1; exact ih1
+    case _ =>
+      have lem : ⊢ ([r#r]A :: Δ) := by constructor; apply h1; apply ih1 r h1 h2
+      replace ih2 := @ih2 ([r#r]A :: Δ) (Term.Ren.lift r) lem (rename_lift r A h2)
       simp at ih2; exact ih2
   case app Γ' f A' B a B' _j1 _j2 j3 ih1 ih2 =>
     simp; constructor
-    case _ => apply ih1 r h
-    case _ => apply ih2 r h
+    case _ => apply ih1 r h1 h2
+    case _ => apply ih2 r h1 h2
     case _ => subst j3; simp
-  case econv Γ' t A' B K _j1 _j2 j3 ih1 ih2 =>
+  case conv Γ' t A' B K _j1 _j2 j3 ih1 ih2 =>
     constructor
-    case _ => apply ih1 r h
-    case _ => apply ih2 r h
-    case _ => apply Term.RedConv.subst; apply j3
-  case iconv Γ' t A' B K _j1 _j2 j3 ih1 ih2 =>
-    constructor
-    case _ => apply ih1 r h
-    case _ => apply ih2 r h
-    case _ => apply Term.RedConv.subst; apply j3
+    case _ => apply ih1 r h1 h2
+    case _ => apply ih2 r h1 h2
+    case _ => apply RedConv.subst; apply j3
 
-  theorem rename_wf (r : Ren) : t ⊢ Γ ->
-    (∀ x, [r#r](Γ d@ x) = Δ d@ (r x)) ->
-    ([r#r]t) ⊢ Δ
-  := by
-  intro j h
-  induction j generalizing Δ r
-  case ax => simp; constructor
-  case var j1 _j2 ih =>
-    have j2 := rename r j1 h
-    simp at *; constructor; rw [h] at j2; exact j2
-    replace ih := ih r h; rw [h _] at ih; exact ih
-  case pi A Γ B _ _ ih1 ih2 =>
-    simp; constructor; apply ih1 r h
-    replace ih2 := @ih2 ([r#r]A :: Δ) (Term.Ren.lift r) (rename_lift r A h); simp at ih2
-    exact ih2
-  case lam A Γ B _ _ ih1 ih2 =>
-    simp; constructor; apply ih1 r h
-    replace ih2 := @ih2 ([r#r]A :: Δ) (Term.Ren.lift r) (rename_lift r A h); simp at ih2
-    exact ih2
-  case app _ _ ih1 ih2 =>
-    simp; constructor; apply ih1 r h; apply ih2 r h
-  case conv _ _ ih1 ih2 =>
-    simp; constructor; apply ih1 r h; apply ih2 r h
+  -- theorem rename_wf (r : Ren) : t ⊢ Γ ->
+  --   (∀ x, [r#r](Γ d@ x) = Δ d@ (r x)) ->
+  --   ([r#r]t) ⊢ Δ
+  -- := by
+  -- intro j h
+  -- induction j generalizing Δ r
+  -- case ax => simp; constructor
+  -- case var j1 _j2 ih =>
+  --   have j2 := rename r j1 h
+  --   simp at *; constructor; rw [h] at j2; exact j2
+  --   replace ih := ih r h; rw [h _] at ih; exact ih
+  -- case pi A Γ B _ _ ih1 ih2 =>
+  --   simp; constructor; apply ih1 r h
+  --   replace ih2 := @ih2 ([r#r]A :: Δ) (Term.Ren.lift r) (rename_lift r A h); simp at ih2
+  --   exact ih2
+  -- case lam A Γ B _ _ ih1 ih2 =>
+  --   simp; constructor; apply ih1 r h
+  --   replace ih2 := @ih2 ([r#r]A :: Δ) (Term.Ren.lift r) (rename_lift r A h); simp at ih2
+  --   exact ih2
+  -- case app _ _ ih1 ih2 =>
+  --   simp; constructor; apply ih1 r h; apply ih2 r h
+  -- case conv _ _ ih1 ih2 =>
+  --   simp; constructor; apply ih1 r h; apply ih2 r h
 
-  theorem weaken B : Γ ⊢ t : A -> (B::Γ) ⊢ ([S]t) : ([S]A) := by
-  intro j; apply rename; exact j
-  case _ => intro x; simp; rw [Term.S_to_rS]; unfold rS; simp
+  -- theorem weaken B : Γ ⊢ t : A -> (B::Γ) ⊢ ([S]t) : ([S]A) := by
+  -- intro j; apply rename; exact j
+  -- case _ => intro x; simp; rw [Term.S_to_rS]; unfold rS; simp
 
-  theorem weaken_wf A : t ⊢ Γ -> ([S]t) ⊢ (A::Γ) := by
-  intro j; apply rename_wf; exact j
-  case _ => intro x; simp; rw [Term.S_to_rS]; unfold rS; simp
+  -- theorem weaken_wf A : t ⊢ Γ -> ([S]t) ⊢ (A::Γ) := by
+  -- intro j; apply rename_wf; exact j
+  -- case _ => intro x; simp; rw [Term.S_to_rS]; unfold rS; simp
 
 
 namespace Fomega.Proof
