Fomega/Proof.lean
@@ -4,48 +4,96 @@ import Fomega.Ctx
 
 namespace Fomega
 
-  inductive Proof : Ctx -> Term -> Term -> Prop
-  | ax :
-    ∀ (f : Nat -> Const), (∀ x, Proof Γ (Γ d@ x) (.const (f x))) ->
-    Proof Γ ★ □
-  | var :
-    Proof Γ (Γ d@ x) (.const K) ->
-    Proof Γ (.bound K x) (Γ d@ x)
-  | pi :
-    Proof Γ A (.const K) ->
-    Proof (A::Γ) B ★ ->
-    Proof Γ (.all mf A B) ★
-  | tpi :
-    Proof Γ A □ ->
-    Proof (A::Γ) B □ ->
-    Proof Γ (.all mf A B) □
-  | lam :
-    Proof Γ (.all mf A B) (.const K) ->
-    Proof (A::Γ) t B ->
-    Proof Γ (.lam mf A t) (.all mf A B)
-  | app :
-    Proof Γ f (.all mf A B) ->
-    Proof Γ a A ->
-    B' = (B β[a]) ->
-    Proof Γ (.app mf f a) B'
-  | conv :
-    Proof Γ t A ->
-    Proof Γ B (.const K) ->
-    A =β= B ->
-    Proof Γ t B
+  inductive JudgmentVariant : Type
+  | prf | wf
 
-  inductive Wf : Term -> Ctx -> Prop
-  | ax : Wf (.const K) Γ
+  @[simp, inline]
+  abbrev JudgmentIndex : JudgmentVariant -> Type
+  | .prf => Term × Term
+  | .wf => Unit
+
+  inductive Judgment : (v : JudgmentVariant) -> Ctx -> JudgmentIndex v -> Prop
+  | nil : Judgment .wf [] ()
+  | cons :
+    Judgment .wf Γ () ->
+    Judgment .prf Γ (A, .const K) ->
+    Judgment .wf (A::Γ) ()
+  | ax :
+    Judgment .wf Γ () ->
+    Judgment .prf Γ (★, □)
   | var :
-    Proof Γ (Γ d@ x) (.const K) ->
-    Wf (Γ d@ x) Γ ->
-    Wf (.bound K x) Γ
-  | pi : Wf A Γ -> Wf B (A::Γ) -> Wf (.all mf A B) Γ
-  | lam : Wf A Γ -> Wf B (A::Γ) -> Wf (.lam mf A B) Γ
-  | app : Wf f Γ -> Wf a Γ -> Wf (.app mf f a) Γ
-  | conv : Wf B Γ -> Wf t Γ -> Wf (.conv 0 B t) Γ
+    Judgment .prf Γ (Γ d@ x, .const K) ->
+    T = Γ d@ x ->
+    Judgment .prf Γ (.bound K x, T)
+  | pi :
+    Judgment .prf Γ (A, .const K) ->
+    Judgment .prf (A::Γ) (B, ★) ->
+    Judgment .prf Γ (.all mf A B, ★)
+  | tpi :
+    Judgment .prf Γ (A, □) ->
+    Judgment .prf (A::Γ) (B, □) ->
+    Judgment .prf Γ (.all mf A B, □)
+  | lam :
+    Judgment .prf Γ (.all mf A B, .const K) ->
+    Judgment .prf (A::Γ) (t, B) ->
+    Judgment .prf Γ (.lam mf A t, .all mf A B)
+  | app :
+    Judgment .prf Γ (f, .all mf A B) ->
+    Judgment .prf Γ (a, A) ->
+    B' = (B β[a]) ->
+    Judgment .prf Γ (.app mf f a, B')
+  | conv :
+    Judgment .prf Γ (t, A) ->
+    Judgment .prf Γ (B, .const K) ->
+    A =β= B ->
+    Judgment .prf Γ (t, B)
+
+
+  notation:170 Γ:170 " ⊢ " t:170 " : " A:170 => Judgment JudgmentVariant.prf Γ (t, A)
+  notation:170 "⊢ " Γ:170 => Judgment JudgmentVariant.wf Γ ()
+
+  @[simp]
+  abbrev all_inversion_idx A B T : JudgmentIndex v :=
+    match v with
+    | .prf => (.all mf A B, T)
+    | .wf => ()
+
+  theorem all_destruct :
+    Γ ⊢ .all mf A B : T ->
+    T =β= .const K ->
+    Γ ⊢ .all mf A B : .const K ∧ (∃ K, Γ ⊢ A : .const K) ∧ (A::Γ) ⊢ B : .const K
+  := by
+  intro j hc
+  generalize tdef : Term.all mf A B = t at *
+  induction j generalizing A B K
+  case ax => simp at tdef
+  case var => simp at tdef
+  case pi Γ' A' K' B' j1 j2 ih1 ih2 =>
+    injection tdef with e1 e2 e3
+    subst e2; subst e3
+    cases K
+    case _ =>
+      apply And.intro; constructor; apply j1; apply j2
+      apply And.intro; exists K'
+      apply j2
+    case _ => exfalso; apply Term.RedConv.type_not_conv_to_kind hc
+  case tpi Γ' A' B' j1 j2 ih1 ih2 =>
+    injection tdef with e1 e2 e3
+    subst e2; subst e3
+    cases K
+    case _ => exfalso; apply Term.RedConv.type_not_conv_to_kind (Term.RedConv.sym hc)
+    case _ =>
+      apply And.intro; constructor; apply j1; apply j2
+      apply And.intro; exists .kind
+      apply j2
+  case lam => simp at tdef
+  case app => simp at tdef
+  case econv Γ t' A' B' _K' h1 _h2 _h3 ih1 _ih2 =>
+    cases t' <;> simp at tdef
+  case iconv Γ t' A' B' _K' h1 _h2 h3 ih1 _ih2 =>
+    cases t' <;> simp at tdef
+    case all m C D =>
+      apply ih1 (Term.RedConv.trans h3 hc)
+      rw [tdef.1, tdef.2.1, tdef.2.2]
 
 end Fomega
-
-notation:170 Γ:170 " ⊢ " t:170 " : " A:170 => Fomega.Proof Γ t A
-notation:170 t:170 " ⊢ " Γ:170 => Fomega.Wf t Γ
