Fomega/PreProof.lean
@@ -4,12 +4,12 @@ import Fomega.Proof
 
 namespace Fomega
 
-  theorem ctx_wf : Γ ⊢ t : A -> ∃ (f:Nat -> Const), ∀ x, Γ ⊢ (Γ d@ x) : (.const (f x)) := by
+  theorem judgment_ctx_wf : Judgment v Γ idx -> ⊢ Γ := by
   intro j
   induction j
-  all_goals (try (case _ ih => apply ih))
-  all_goals (try (case _ ih _ => apply ih))
-  case ax f h _ => exists f
+  case nil => constructor
+  case cons j1 j2 _ _ => constructor; apply j1; apply j2
+  all_goals try simp [*]
 
   inductive IsPreProof : Term -> Prop where
   | ax : IsPreProof (.const K)
@@ -17,7 +17,6 @@ namespace Fomega
   | all : IsPreProof A -> IsPreProof B -> IsPreProof (.all mf A B)
   | lam : IsPreProof A -> IsPreProof t -> IsPreProof (.lam mf A t)
   | app : IsPreProof f -> IsPreProof a -> IsPreProof (.app mf f a)
-  | conv : IsPreProof B -> IsPreProof t -> IsPreProof (.conv 0 B t)
 
   namespace IsPreProof
     theorem from_subst : IsPreProof ([σ]t) -> IsPreProof t := by
@@ -25,8 +24,6 @@ namespace Fomega
     induction t generalizing σ <;> (try (simp at j; cases j))
     case bound K x => constructor
     case _ => constructor
-    case _ ih1 ih2 j1 j2 =>
-      constructor; apply ih1 j1; apply ih2 j2
     case _ ih1 ih2 j1 j2 =>
       constructor; apply ih1 j1; apply ih2 j2
     case _ ih1 ih2 j1 j2 =>
@@ -48,8 +45,6 @@ namespace Fomega
       replace ih2 := @ih2 (Term.Ren.lift r)
       simp at ih2; exact ih2
     case app _j1 _j2 ih1 ih2 =>
-      constructor; apply ih1; apply ih2
-    case conv _j1 _j2 ih1 ih2 =>
       constructor; apply ih1; apply ih2
 
     theorem lift : (∀ n s, σ n = .replace s -> IsPreProof s) -> ∀ n s, ^σ n = .replace s -> IsPreProof s := by
@@ -83,8 +78,6 @@ namespace Fomega
       simp at ih2; exact ih2
     case app _j1 _j2 ih1 ih2 =>
       constructor; apply ih1 h; apply ih2 h
-    case conv _j1 _j2 ih1 ih2 =>
-      constructor; apply ih1 h; apply ih2 h
 
     theorem beta : IsPreProof b -> IsPreProof t -> IsPreProof (b β[t]) := by
     simp; intro j1 j2
@@ -95,34 +88,34 @@ namespace Fomega
       subst eq; exact j2
     case _ => exact j1
 
-    theorem from_proof : Γ ⊢ t : A -> IsPreProof t := by
-    intro j; induction j
-    case ax => constructor
-    case var => constructor
-    case pi _j1 _j2 ih1 ih2 => constructor <;> simp [*]
-    case tpi => constructor <;> simp [*]
-    case lam j1 _j2 ih1 ih2 => constructor; cases ih1; all_goals simp [*]
-    case app => constructor <;> simp [*]
-    case econv => constructor <;> simp [*]
-    case iconv => simp [*]
+    -- theorem from_proof : Γ ⊢ t : A -> IsPreProof t := by
+    -- intro j; induction j
+    -- case ax => constructor
+    -- case var => constructor
+    -- case pi _j1 _j2 ih1 ih2 => constructor <;> simp [*]
+    -- case tpi => constructor <;> simp [*]
+    -- case lam j1 _j2 ih1 ih2 => constructor; cases ih1; all_goals simp [*]
+    -- case app => constructor <;> simp [*]
+    -- case econv => constructor <;> simp [*]
+    -- case iconv => simp [*]
 
-    theorem from_proof_type : t ⊢ Γ -> Γ ⊢ t : A -> IsPreProof A := by
-    intro h j; induction j
-    case ax => constructor
-    case var =>
-      cases h
-      case _ h => apply (from_proof h)
-    case pi => constructor
-    case tpi => constructor
-    case lam j _ _ _ => apply from_proof j
-    case app _j1 j2 j3 ih1 _ih2 =>
-      cases h
-      case _ h1 h2 =>
-        cases (ih1 h1)
-        case _ p1 p2 =>
-        subst j3; apply beta p2 (from_proof j2)
-    case econv j _ _ _ => apply from_proof j
-    case iconv j _ _ _ => apply from_proof j
+    -- theorem from_proof_type : t ⊢ Γ -> Γ ⊢ t : A -> IsPreProof A := by
+    -- intro h j; induction j
+    -- case ax => constructor
+    -- case var =>
+    --   cases h
+    --   case _ h => apply (from_proof h)
+    -- case pi => constructor
+    -- case tpi => constructor
+    -- case lam j _ _ _ => apply from_proof j
+    -- case app _j1 j2 j3 ih1 _ih2 =>
+    --   cases h
+    --   case _ h1 h2 =>
+    --     cases (ih1 h1)
+    --     case _ p1 p2 =>
+    --     subst j3; apply beta p2 (from_proof j2)
+    -- case econv j _ _ _ => apply from_proof j
+    -- case iconv j _ _ _ => apply from_proof j
 
   end IsPreProof
 
